doc-src/TutorialI/Recdef/Nested1.thy
@@ -21,7 +21,7 @@ text{*\noindent
 Remember that function @{term size} is defined for each \isacommand{datatype}.
 However, the definition does not succeed. Isabelle complains about an
 unproved termination condition
-@{term[display]"t : set ts --> size t < Suc (term_list_size ts)"}
+@{prop[display]"t : set ts --> size t < Suc (term_list_size ts)"}
 where @{term set} returns the set of elements of a list
 and @{text"term_list_size :: term list \<Rightarrow> nat"} is an auxiliary
 function automatically defined by Isabelle
